WIP: new induction idea by Mathias

dataplane/Correctness/Produces.thy
@@ -721,7 +721,7 @@ lemma dataplane_tracker_inv_produces_drops:
             apply (metis (no_types, lifting) change_multiplicities_append_alt change_multiplicities_comm)
             done
           done
-        subgoal for nid' xs
+                      subgoal for nid' xs
           unfolding changes_above_impl_inv_def
           apply safe
           subgoal for l t m
@@ -731,131 +731,258 @@ lemma dataplane_tracker_inv_produces_drops:
               apply (subst (asm) extract_progress_def)
               apply (clarsimp simp add: image_iff split_beta Misc.set_map_filter split: option.splits; hypsubst_thin?)
               subgoal for p' m
-                apply (subst change_multiplicities_extract_prog_updates[where nid=nid])
-                  apply assumption+
-                apply (cases "\<exists> l t' s. (node l = nid \<longrightarrow> is_Trg (port l)) \<and> t \<ge> t' -+- s \<and> s \<in>\<^sub>A graph.path_weight (summ sg) l (Loc nid' (Trg p')) \<and> frontier_less_equal (frontier (c_pts (change_multiplicities (summ sg) (extract_prog xs (graph_to_nxt (summ sg)) os) (pt_tr sg)) l)) t'")
+                apply (frule conjunct1[OF conjunct2[OF prems(15)[unfolded produ_consu_inter_supported_def]], rule_format])
+                apply (cases "\<exists> nid'' p''. graph_to_nxt (summ sg) (nid'', p'') = Some (nid', p')")
                 subgoal
                   apply clarsimp
-                  subgoal for l' t' s
-                    apply (cases "node l' = nid")
+                  subgoal for nid'' p''
+                    apply (cases "nid'' \<in> set xs")
                     subgoal
-                      apply simp
-                      apply (rule frontier_less_equal_trans[rotated])
-                      apply assumption
-                      apply (rule frontier_less_equal_ifrontierI[OF D, of s l'])
-                      apply assumption
-                      apply (clarsimp simp add: c_pts_change_multiplicities)
-                      apply (subst (3) filter_False)
+                      apply (rule frontier_less_equal_ifrontierI[OF D, of 0 "Loc nid' (Trg p')", simplified])
                       subgoal
-                        apply (cases l'; simp)
-                        apply (auto simp add: Misc.set_map_filter extract_prog_def extract_progress_def image_iff obtain_progress_def split: option.splits)
-                        done
+                        sorry
                       subgoal
-                        apply simp
-                        apply (subgoal_tac "\<forall> t. zcount (zmset (map snd (filter (\<lambda>(l'a, t, d). l' = l'a) (List.map_filter (\<lambda>(p, t, m). case graph_to_nxt (summ sg) (node l', p) of None \<Rightarrow> None | Some (nid', p') \<Rightarrow> Some (Loc nid' (Trg p'), t, m)) produs)))) t \<ge> 0")
+                        apply (cases "nid'' = nid")
                         subgoal
-                          by (metis (no_types, lifting) ab_semigroup_add_class.add_ac(1) frontier_below_eq_frontier_plus_pos frontier_less_equal_le_trans)
-                        subgoal
-                  apply (auto simp add: Misc.set_map_filter zcount_sum filter_empty_conv intro!: zcount_zmset_ge_0I zmset_emptyI ordered_comm_monoid_add_class.sum_nonneg split: option.splits)
-                          using prems(12)[unfolded change_deltas_inv_def]
-                          apply (metis graph_to_nxt_Some_alt old.prod.case temp(2,5) zle_add1_eq_le zless_add1_eq)
+                          apply hypsubst_thin
+                        apply (subst change_multiplicities_extract_prog_obtain_progress_remove1_append[where nid=nid])
+                        apply simp_all
+                        apply (clarsimp simp add: c_pts_change_multiplicities obtain_progress_def extract_progress_def filter_map comp_def split_beta split: option.splits)
+                          apply (subst (3) filter_False)
+                          subgoal
+                            apply (auto simp add: obtain_progress_def Misc.set_map_filter extract_prog_def extract_progress_def split: option.splits)
+                            using temp(5)[unfolded graph_summar_nt_def]
+                            apply (metis (no_types, lifting) Pair_inject domI in_op_conn_graph_to_nxt_iff inj_on_eq_iff op_conn.simps)
+                            done
+                          apply (clarsimp simp add: monoid_add_class.sum_list_distinct_conv_sum_set split_beta zmset_concat comp_def)
+                          apply (subgoal_tac "
+ (\<Sum>x\<in>UNIV. zmset (map snd (filter (\<lambda>(p'', ab). graph_to_nxt (summ sg) (fst x, p'') = Some (nid', p') \<and> snd x = p'') (produ (os (fst x)))))) = 
+  zmset
+          (map snd
+            (filter (\<lambda>(l', t, d). Loc nid' (Trg p') = l') (List.map_filter (\<lambda>(p, t, m). case graph_to_nxt (summ sg) (nid, p) of None \<Rightarrow> None | Some (nid', p') \<Rightarrow> Some (Loc nid' (Trg p'), t, m)) (produ (os nid)))))")
+                          defer
+                          subgoal
+                            apply (subst comm_monoid_add_class.sum.subset_diff[of "{(nid, p'')}"])
+                            apply simp_all
+                            apply (subst comm_monoid_add_class.sum.neutral)
+                            subgoal
+                              apply clarsimp
+                              using temp(5)[unfolded graph_summar_nt_def]
+                              apply (smt (verit, best) case_prodE domI filter_empty_conv inj_on_def list.map_disc_iff prod.inject zmset_emptyI)
+                              done
+                            apply simp
+                            apply (subst map_snd_filter_List_map_filter)
+                              apply assumption
+                            using temp(5)[unfolded graph_summar_nt_def] apply simp_all
+                            done
+                          subgoal
+                            apply simp
+                            apply (rule frontier_less_equal_zcount_pos)
+                            apply (simp flip: add.assoc)
+                            apply (rule ordered_comm_monoid_add_class.add_pos_nonneg)
+                             apply simp_all
+                            apply (rule zcount_zmset_ge_0I)
+                            apply (auto simp add:  Misc.set_map_filter split: option.splits)
+                            using temp(2) temp(5)[unfolded graph_summar_nt_def] apply (smt (verit) in_op_conn_graph_to_nxt_iff old.prod.case op_conn.simps)
+                            done
                           done
-                        done
-                      done
-                    subgoal
-                      apply simp
-                      apply (rule frontier_less_equal_trans[rotated])
-                      apply assumption
-                      apply (rule frontier_less_equal_ifrontierI[OF D, of s l'])
-                      apply assumption
-                      apply (clarsimp simp add: c_pts_change_multiplicities)
-                      apply (subst (3) filter_False)
-                      subgoal
-                        apply (cases l'; simp)
-                        done
-                      subgoal 
-                        apply (subgoal_tac "\<forall> t. zcount (zmset (map snd (filter (\<lambda>(l'a, t, d). l' = l'a) (List.map_filter (\<lambda>(p, t, m). case graph_to_nxt (summ sg) (nid, p) of None \<Rightarrow> None | Some (nid', p') \<Rightarrow> Some (Loc nid' (Trg p'), t, m)) produs)))) t \<ge> 0")
                         subgoal
+                        apply (subst change_multiplicities_extract_prog_obtain_progress_remove1_append[where nid=nid''])
+                        apply simp_all
+                        apply (clarsimp simp add: c_pts_change_multiplicities obtain_progress_def extract_progress_def filter_map comp_def split_beta split: option.splits)
+                          apply (subst (2) filter_False)
+                          subgoal
+                            apply (auto simp add: obtain_progress_def Misc.set_map_filter extract_prog_def extract_progress_def split: option.splits)
+                            using temp(5)[unfolded graph_summar_nt_def]
+                             apply (metis (no_types, lifting) domI in_op_conn_graph_to_nxt_iff inj_on_eq_iff op_conn.simps prod.simps(1))+
+                            done
                           apply simp
-                          apply (metis (no_types, lifting) ab_semigroup_add_class.add_ac(1) frontier_below_eq_frontier_plus_pos frontier_less_equal_le_trans)
-                          done
-                        subgoal
-                          apply (auto simp add: Misc.set_map_filter zcount_sum filter_empty_conv intro!: zcount_zmset_ge_0I zmset_emptyI ordered_comm_monoid_add_class.sum_nonneg split: option.splits)
-                          using prems(12)[unfolded change_deltas_inv_def]
-                          apply (metis graph_to_nxt_Some_alt old.prod.case temp(2,5) zle_add1_eq_le zless_add1_eq)
+                          apply (clarsimp simp add: monoid_add_class.sum_list_distinct_conv_sum_set split_beta zmset_concat comp_def)
+                          apply (subst (asm) comm_monoid_add_class.sum.subset_diff[of "{(nid'', p'')}"])
+                            apply simp_all
+                            apply (subst (asm) comm_monoid_add_class.sum.neutral)
+                            subgoal
+                              apply clarsimp
+                              using temp(5)[unfolded graph_summar_nt_def]
+                              apply (smt (verit, best) case_prodE domI filter_empty_conv inj_on_def list.map_disc_iff prod.inject zmset_emptyI)
+                              done
+                            apply simp
+                            apply (subst map_snd_filter_List_map_filter)
+                              apply assumption
+                            using temp(5)[unfolded graph_summar_nt_def] apply simp
+                            apply (simp flip: zcount_union)
+                            apply (drule zcount_gt_0_in_frontierD)
+                            apply clarsimp
+                            apply (subst (2) filter_False)
+                            using frontier_less_equal_iff2 apply auto
+                            done
                           done
                         done
-                      done
-                    done
-                  done
-                subgoal
-                  apply auto
-                using prems(14)[unfolded extract_prog_changes_above_impl_inv_def changes_above_impl_inv_def, rule_format, of xs nid' "(Loc nid' (Trg p'), t, -m)"] apply -
-                apply simp
-                apply (drule meta_mp)
-                subgoal
-                  unfolding extract_progress_def obtain_progress_def
-                  apply simp
-                  apply force
-                  done
-                subgoal
-                  apply (drule frontier_less_equal_ifrontierE[OF _ D])
-                  apply clarsimp
-                  subgoal for l s t'
-                    apply hypsubst_thin
-                      apply (cases "\<exists> p. l = Loc nid (Src p)")
-                       apply clarsimp
-                      subgoal for p
-                        apply hypsubst_thin
-                        oops
+                      subgoal
+                        apply (cases "nid'' = nid")
+                        subgoal
+                          by auto
+                        subgoal
+                      apply (subst change_multiplicities_extract_prog_updates[where nid=nid])
+                            apply assumption+
+                          apply (simp add: map_concat comp_def)
+                          apply (subgoal_tac "0 < zcount (c_pts (pt_tr sg) (Loc nid' (Trg p'))) t \<or> 0 < zcount (zmset (concat (map (\<lambda>(nid'a, p'a). map snd (filter (\<lambda>(p'', ab). graph_to_nxt (summ sg) (nid'a, p'') = Some (nid', p') \<and> p'a = p'') (produ (os nid'a)))) enum_class.enum))) t")
+                          defer
+                          subgoal
+                            by auto
+                          subgoal
+                            apply (elim disjE)
+                            subgoal
+                              apply (rule frontier_less_equal_ifrontierI[OF D, of 0 "Loc nid' (Trg p')", simplified])
+                              subgoal
+                                sorry
+                              subgoal
+                                apply (simp add: c_pts_change_multiplicities)
+                                apply (subst filter_False)
+                                subgoal
+                                  unfolding extract_progress_def obtain_progress_def extract_prog_def
+                                  apply (auto simp add:  Misc.set_map_filter split: option.splits)
+                                  using temp(5)[unfolded graph_summar_nt_def]
+                                   apply (metis (no_types, lifting) domI in_op_conn_graph_to_nxt_iff inj_on_eq_iff op_conn.simps prod.simps(1))+
+                                  done
+                                apply (subst filter_False)
+                                subgoal
+                                  unfolding extract_progress_def obtain_progress_def extract_prog_def
+                                  apply (auto simp add: Misc.set_map_filter split: option.splits)
+                                  using temp(5)[unfolded graph_summar_nt_def]
+                                  apply (metis (no_types, lifting) domI in_op_conn_graph_to_nxt_iff inj_on_eq_iff op_conn.simps prod.simps(1))
+                                  done
+                                subgoal
+                                  apply simp
+                                  apply (metis frontier_less_equal_zcount_pos)
+                                  done
+                                done
+                              done
+                            subgoal
+                              apply (clarsimp simp add: zcount_sum monoid_add_class.sum_list_distinct_conv_sum_set  comp_def zmset_concat split_beta)
+                              apply (subgoal_tac "\<exists> m. (p'', t, m) \<in> set (produ (os nid''))")
+                               defer
+                              subgoal
+                                apply (drule sum_pos_ex_elem_pos)
+                                apply clarsimp
+                                apply (drule zcount_zmset_gt_0_set_Ex)
+                                apply clarsimp
+                                using temp(5)[unfolded graph_summar_nt_def]
+                                apply (metis (mono_tags, lifting) domI fst_eqD inv_on_f_f snd_eqD)
+                                done
+                              subgoal
+                                apply clarsimp
+                                subgoal for m'
+                                  thm prems(15)
+
+                                  apply (drule conjunct1[OF prems(15)[unfolded produ_consu_inter_supported_def], rule_format])
+                                  apply (elim disjE)
+                                  subgoal
+                                    apply (rule frontier_less_equal_ifrontierI[of _ 0 "Loc nid'' (Src p'')", simplified, OF D])
+                                        subgoal sorry
+                                        apply (simp add: change_multiplicities_append_alt)
+                                        apply (clarsimp simp add: c_pts_change_multiplicities)
+                                        apply (subst (2) filter_False)
+                                        subgoal
+                                          by (auto simp add: Misc.set_map_filter split: option.splits)
+                                        apply simp
+                                        apply (subst (1) filter_False)
+                                        subgoal
+                                          by (auto simp add: Misc.set_map_filter map_concat extract_prog_def extract_progress_def split_beta image_iff del: disjCI split: option.splits)
+                                        apply simp
+                                        using frontier_less_equal_trans frontier_less_equal_zcount_pos apply blast
+                                        done
+                                  subgoal
+                                    apply clarsimp
+                                    subgoal for m''
+                                      apply (drule conjunct2[OF conjunct2[OF prems(15)[unfolded produ_consu_inter_supported_def]], rule_format])
+                                      apply clarsimp
+                                      apply (elim disjE)
+                                      subgoal for t'
+                                        apply (rule frontier_less_equal_ifrontierI[of _ 0 "Loc nid'' (Src p'')", simplified, OF D])
+                                        subgoal sorry
+                                        apply (simp add: change_multiplicities_append_alt)
+                                        apply (clarsimp simp add: c_pts_change_multiplicities)
+                                        apply (subst (2) filter_False)
+                                        subgoal
+                                          by (auto simp add: Misc.set_map_filter split: option.splits)
+                                        apply simp
+                                        apply (subst (1) filter_False)
+                                        subgoal
+                                          by (auto simp add: Misc.set_map_filter map_concat extract_prog_def extract_progress_def split_beta image_iff del: disjCI split: option.splits)
+                                        apply simp
+                                        using frontier_less_equal_trans frontier_less_equal_zcount_pos apply blast
+                                        done
+                                      subgoal for t'
+                                        apply clarsimp
+
+                                        oops
 
 
 
 function find_timestamp where
-  "find_timestamp c su S (l :: 'loc :: {enum}) t =
-   (if l \<in> S then {}
-    else if \<exists> t'\<le>t. zcount (c_pts c l) t' > 0 
-    then {l} 
-    else
-    let L = {(l', t'). \<exists> s. s \<in>\<^sub>A su l' l \<and> t = t' -+- s} in \<Union> ((\<lambda> (l', t'). find_timestamp c su (insert l S) l' t') ` L))"
+  "find_timestamp su P T (l :: 'loc :: {enum}) t =
+   (if P l t then {l} else
+    if t \<in> set (T l) then let LT = {(l', t'). \<exists> s. s \<in>\<^sub>A su l' l \<and> t = t' -+- s} in \<Union> ((\<lambda> (l', t'). find_timestamp su P (T(l := filter ((\<noteq>) t) (T l))) l' t') ` LT)
+    else {})"
   by auto
 termination
-  apply (relation "measure (\<lambda>(c, su, S, l, t). card ((UNIV :: 'loc set) - S))")
+  apply (relation "measure (\<lambda>(su, P, T, l, t). sum (\<lambda> l'. card (set (T l'))) UNIV)")
    apply simp
-  apply clarsimp
-  apply (rule diff_Suc_less)
-  apply (simp add: card_gt_0_iff)
-  apply blast
+  apply (clarsimp split: if_split)
+  apply (rule sum_strict_mono_ex1)
+    apply (auto simp add: card_mono intro!: psubset_card_mono)
   done
 
-lemma find_timestamp_sound:
-  assumes G: "Graph.graph su"
-  shows "l' \<in> find_timestamp c su S l t \<Longrightarrow>
-   (\<exists> s t'. s \<in>\<^sub>A graph.path_weight su l' l \<and> s -+- t' \<le> t \<and> zcount (c_pts c l') t' > 0)"
-  using assms
-  apply (induction c su S l t arbitrary: l' rule: find_timestamp.induct)
-  subgoal for c su S l t l'
-    apply (subst (asm) (2) find_timestamp.simps)
-    apply (split if_splits)
-    subgoal by simp
-    apply (split if_splits)
-    subgoal for t'
-      apply clarsimp
-      apply hypsubst_thin
-      subgoal
-        apply (rule exI[of _ 0])
-        apply (intro conjI)
-        apply (meson graph.path_weight_refl)
-        apply (rule exI[of _ t'])
-         apply simp
-        done
-      done
+declare find_timestamp.simps[simp del]
+
+definition "backtracks su P T = (\<forall> t l. t \<in> set (T l) \<longrightarrow> (\<exists> l' t' s. l \<noteq> l' \<and> s \<in>\<^sub>A su l' l \<and> t = t' -+- s \<and> t' \<in> set (T l')) \<or> P l t)"
+
+lemma find_timestamp_non_empty:
+  "backtracks su P T \<Longrightarrow>
+   t \<in> set (T l) \<Longrightarrow>
+   find_timestamp su P T l t \<noteq> {}"
+  apply (induction su P T l t arbitrary: rule: find_timestamp.induct)
+  subgoal for su P T l t
+    apply (subst find_timestamp.simps)
+    apply (auto split: if_splits)
     subgoal
-      apply clarsimp
-      subgoal for l'' t'' s_edge
-        oops
+      apply (subst (asm) (2) backtracks_def)
+      apply (drule spec2, drule mp, assumption)
+      apply (auto split: if_splits)
+      apply (intro exI conjI)
+        apply assumption
+       apply (rule refl)
+      subgoal premises prems for l' t' s
+        using prems(2-) apply -
+        apply (rule prems(1))
+           apply (rule refl)
+        using prems apply blast
+          apply (rule refl)
+        subgoal
+        apply (auto 0 0 simp add: backtracks_def)
+        subgoal for t''
+          apply hypsubst_thin
+          apply (rule exI[of _ l'])
+          apply (intro conjI impI)
+           apply auto
+          apply (rule exI[of _ t'])
+          apply (rule exI[of _ s])
+          apply (intro conjI)
+            apply simp
+          apply simp
 
 
+
+
+
+
+        term Graph.graph.path
+
+lemma (in Graph.graph) foo:
+  "(\<forall> v \<in> (V :: 'vtx set). \<not> P v) \<Longrightarrow>
+   (\<forall> v \<in> (V :: 'vtx set). \<exists> xs. path w v xs) \<Longrightarrow>
+   \<exists> w' xs. P w' \<and> path w w' xs"
 
 lemma backtrack_consu_to_non_nid:
   assumes P: "produ_consu_inter_supported (graph_to_nxt su) os c"
